---
title: "Analytical Solution with Independent Return"
header-includes:
  - \usepackage{amssymb, amsmath, amsthm}
fontsize: 12pt
output: 
  bookdown::pdf_document2:
    toc: False
---

```{r setup, include=FALSE}
knitr::opts_chunk$set(echo = TRUE)
```

$W_t$ is the wealth just after consumption is deducted from the portfolio. Its evolution follows

$$\begin{aligned}W_{t+1} &= (W_t-\beta_t)\cdot R^f +\beta_t \cdot R^r_t - C_{t+1}\\ &=W_t\cdot R^f + \beta_t(R^r_t-R^f)-C_{t+1}\end{aligned}$$

where

* $R^f$ is the accumulation factor for risk free asset from time $t$ to $t+1$
* $R^r_t$ is the accumulation factor for the risky portfolio from time $t$ to $t+1$
* $\beta_t$ is the amount of wealth invested in the risky portfolio at time $t$
* $C_{t+1}$ is the consumption made at time $t+1$

Value function at time $0$: 

$$V_0(W_0) = \min_{\{C_t\}^T_{t=1}, \{\beta_t\}^{T-1}_{t=0}}E[\sum^{T}_{t=1}\delta^t \cdot(C^2_{t} - 2\lambda C_{t})+\delta^T\cdot (W_T^2 - 2\lambda W_T)]$$

with terminal condition 

$$V_T(W_T) =W_T^2 - 2\lambda W_T$$

where 

* $\lambda$ is added for the convenience of calculation

Value function at time $t$:

$$\begin{aligned}V_t(W_t) &= \min_{\{C_s\}^T_{s=t}, \{\beta_s\}^{T-1}_{s=t}}E[\sum^{T}_{s=t+1}\delta^s \cdot(C^2_{s} - 2\lambda C_{s})+\delta^T\cdot (W_T^2 - 2\lambda W_T)]\\ &=\min_{\{C_s\}^T_{s=t}, \{\beta_s\}^{T-1}_{s=t}}E[\sum^{T}_{s=t+1}\delta^s \cdot((C_s-\lambda)^2-\lambda^2)+\delta^T\cdot ((W_T-\lambda)^2 -\lambda^2)]\end{aligned}$$

The second equality comes from completion of squares.


<!-- $$\left\{\begin{array}{ccc} Z_t=\left(\begin{array}{c}C_t\\ \beta_t\end{array}\right), & S_t=\left(\begin{array}{c}W_t\\ Y_t\end{array}\right), & J=\left(\begin{array}{c}2\lambda\\ r\end{array}\right) \\ \Roman{1}=\left(\begin{array}{c}C_t\\ \beta_t\end{array}\right), & S_t=\left(\begin{array}{c}W_t\\ Y_t\end{array}\right), & J=\left(\begin{array}{c}2\lambda\\ r\end{array}\right)\end{array}\right.$$ -->

Define

$$\widetilde{W_t} = W_t - \lambda\ \ \ \ \ \ \ \ c_t=C_t-\lambda$$



Then the evolution of wealth becomes

$$\begin{aligned}\widetilde{W}_{t+1} &=\widetilde{W}_t\cdot R^f + \beta_t(R^r_t-R^f)-c_{t+1}+(R^f-2)\cdot\lambda\end{aligned}$$

After the transformation, the value function at time $t$ and terminal condition becomes 

$$\left\{\begin{array}{l}V_t(W_t)=\min_{\{C_s\}^T_{s=t}, \{\beta_s\}^{T-1}_{s=t}}E[\sum^{T}_{s=t+1}\delta^{s-t} \cdot(c_s^2-\lambda^2)+\delta^{T-t}\cdot (\widetilde{W}_T^2 -\lambda^2)]\\ \\ V_T(W_T) = \widetilde{W}_T^2 - \lambda^2\end{array} \right.$$


Now define

$$J_t = \left[\begin{array}{c}R^r_t-R^f\\ -1\end{array}\right]\ \ \ \ \ Z_t = \left[\begin{array}{c}\beta_t\\ c_{t+1}\end{array}\right]\ \ \ \ \ \mathbb{I}^{22} = \left[\begin{array}{cc}0 & 0\\ 0 & 1\end{array}\right]$$

The evolution of wealth becomes

$$\begin{aligned}\widetilde{W}_{t+1} &= \widetilde{W}_t\cdot R^f+J_t^\prime Z_t +(R^f-2)\cdot \lambda\end{aligned}$$

The value function at time $t$ and terminal condition:

$$\left\{\begin{array}{l}V_t(W_t)=\min_{\{C_s\}^T_{s=t}, \{\beta_s\}^{T-1}_{s=t}}E[\sum^{T-1}_{s=t}\delta^{s+1-t} \cdot(Z_t^\prime \mathbb{I}^{22} Z_t-\lambda^2)+\delta^{T-t}\cdot (\widetilde{W}_T^2 -\lambda^2)]\\ \\ V_T(W_T) = \widetilde{W}_T^2 - \lambda^2\end{array} \right.$$

The Bellman equation for this problem would be

$$\begin{aligned}V_t(W_t)&=\min_{\{C_s\}^T_{s=t}, \{\beta_s\}^{T-1}_{s=t}}E[\sum^{T-1}_{s=t}\delta^{s+1-t} \cdot(Z_t^\prime \mathbb{I}^{22} Z_t-\lambda^2)+\delta^{T-t}\cdot (\widetilde{W}_T^2 -\lambda^2)]\\ &=\min_{\{C_s\}^T_{s=t}, \{\beta_s\}^{T-1}_{s=t}}E[\delta \cdot(Z_t^\prime \mathbb{I}^{22} Z_t-\lambda^2)+\sum^{T-1}_{s=t+1}\delta^{s+1-t} \cdot(Z_s^\prime \mathbb{I}^{22} Z_s-\lambda^2)+\delta^{T-t}\cdot (\widetilde{W}_T^2 -\lambda^2)] \\ & =\min_{\{C_s\}^T_{s=t}, \{\beta_s\}^{T-1}_{s=t}}E[\delta \cdot(Z_t^\prime \mathbb{I}^{22} Z_t-\lambda^2)+E[\sum^{T-1}_{s=t+1}\delta^{s+1-t} \cdot(Z_s^\prime \mathbb{I}^{22} Z_s-\lambda^2)+\delta^{T-t}\cdot (\widetilde{W}_T^2 -\lambda^2)]]\\ & =\min_{\{C_s\}^T_{s=t}, \{\beta_s\}^{T-1}_{s=t}}E[\delta \cdot(Z_t^\prime \mathbb{I}^{22} Z_t-\lambda^2)+\delta \cdot E[V_{t+1}(W_{t+1})]] \end{aligned}$$

The third equality comes from Law of Iterated Expection conditional on the known information at time t

















